Imp/Stmt/BigStep.lean
@@ -1,0 +1,464 @@
+import Imp.Expr
+import Imp.Expr.Eval
+import Imp.Stmt
+import Imp.Stmt.Delab
+import Imp.Stmt.Optimize
+
+namespace Imp
+
+/--
+Truthiness: the result of evaluating an expression is "truthy" if it's defined and non-zero.
+-/
+def Truthy (v : Option Value) : Prop :=
+  match v with
+  | some v => v ≠ 0
+  | none => False
+
+instance : Decidable (Truthy v) :=
+  match v with
+  | some v =>
+    if h : v ≠ 0 then .isTrue h else .isFalse h
+  | none => .isFalse id
+
+@[simp]
+theorem Truthy.some_nonzero : Truthy (some v) = (v ≠ 0) := by
+  simp [Truthy]
+
+@[simp]
+theorem Truthy.not_none : Truthy none = False := by
+  simp [Truthy]
+
+@[simp]
+theorem Truthy.eval_const : Truthy (Expr.eval ρ (.const v)) = (v ≠ 0) := by
+  simp [Truthy, Expr.eval]
+
+/--
+Falsiness: the result of evaluating an expression is "falsy" if it's 0
+-/
+def Falsy (v : Option Value) : Prop := v = some 0
+
+@[simp]
+theorem Falsy.eval_const : Falsy (Expr.eval ρ (.const v)) = (v = 0) := by
+  simp [Falsy, Expr.eval]
+
+@[simp]
+theorem Falsy.some_zero : Falsy (some v) = (v = 0) := by
+  simp [Falsy]
+
+@[simp]
+theorem Falsy.not_none : Falsy none = False := by
+  simp [Falsy]
+
+@[simp]
+theorem Falsy.some_const : Falsy (some (BitVec.ofNat _ n)) → (n % 2 ^ 32 = 0) := by
+  simp [Falsy, BitVec.ofNat, ← Fin.val_inj]
+
+instance : Decidable (Falsy v) := inferInstanceAs (Decidable (v = some 0))
+
+theorem Truthy.not_falsy : Truthy v → ¬Falsy v := by
+  intro h1 h2
+  simp [Truthy, Falsy] at *
+  cases v <;> simp at * <;> contradiction
+
+
+namespace Stmt
+
+
+inductive BigStep : Env → Stmt → Env → Prop where
+  | skip :
+    BigStep ρ (imp {skip;}) ρ
+  | seq :
+    BigStep ρ s1 ρ' → BigStep ρ' s2 ρ'' →
+    BigStep ρ (imp{ ~s1 ~s2}) ρ''
+  | assign :
+    e.eval ρ = some v →
+    BigStep ρ (imp {~x := ~e;}) (ρ.set x v)
+  | ifTrue :
+    Truthy (c.eval ρ) → BigStep ρ s1 ρ' →
+    BigStep ρ (imp {if (~c) {~s1} else {~s2}}) ρ'
+  | ifFalse :
+    Falsy (c.eval ρ) → BigStep ρ s2 ρ' →
+    BigStep ρ (imp {if (~c) {~s1} else {~s2}}) ρ'
+  | whileTrue :
+    Truthy (c.eval ρ) →
+    BigStep ρ body ρ' →
+    BigStep ρ' (imp {while (~c) {~body}}) ρ'' →
+    BigStep ρ (imp {while (~c) {~body}}) ρ''
+  | whileFalse :
+    Falsy (c.eval ρ) →
+    BigStep ρ (imp {while (~c) {~body}}) ρ
+
+attribute [simp] BigStep.skip
+
+theorem BigStep.unique : BigStep ρ s ρ' → BigStep ρ s ρ'' → ρ' = ρ'' := by
+  intro h1 h2
+  induction h1 generalizing ρ'' with
+  | «skip» => cases h2; rfl
+  | seq _s1 _s2 ih1 ih2 =>
+    cases h2 with
+    | seq s1' s2' =>
+      have := ih1 s1'
+      subst this
+      apply ih2 s2'
+  | assign isVal =>
+    cases h2 with
+    | assign isVal' =>
+      rw [isVal] at *
+      subst_eqs
+      rfl
+  | ifTrue isTrue _stepTrue ih =>
+    cases h2 with
+    | ifTrue isTrue' stepTrue' =>
+      exact ih stepTrue'
+    | ifFalse isFalse =>
+      have := isTrue.not_falsy
+      contradiction
+  | ifFalse isFalse _stepFalse ih =>
+    cases h2 with
+    | ifTrue isTrue' stepTrue' =>
+      have := isTrue'.not_falsy
+      contradiction
+    | ifFalse isFalse' stepFalse' =>
+      exact ih stepFalse'
+  | whileTrue isTrue _stepBody _stepLoop ihBody ihLoop =>
+    cases h2 with
+    | whileTrue isTrue' stepBody' stepLoop' =>
+      have := ihBody stepBody'
+      subst this
+      exact ihLoop stepLoop'
+    | whileFalse isFalse' =>
+      have := isTrue.not_falsy
+      contradiction
+  | whileFalse isFalse =>
+    cases h2 with
+    | whileTrue isTrue' stepBody' stepLoop' =>
+      have := isTrue'.not_falsy
+      contradiction
+    | whileFalse isFalse' =>
+      rfl
+
+
+
+
+
+/--
+`swap` terminates, and the resulting environment contains swapped inputs.
+-/
+example : ∃ρ', BigStep (Env.init 0 |>.set "x" 5 |>.set "y" 22) swap ρ' ∧ ρ'.get "x" = 22 ∧ ρ'.get "y" = 5 := by
+  unfold swap
+  apply Exists.intro
+  constructor
+  . apply BigStep.seq
+    . apply BigStep.assign
+      simp [Expr.eval, Env.get, Env.set]
+      rfl
+    . apply BigStep.seq
+      . apply BigStep.assign
+        simp [Expr.eval, Env.get, Env.set]
+        rfl
+      . simp
+        apply BigStep.assign
+        simp [Expr.eval, Env.get, Env.set]
+        rfl
+  . simp [Env.get, Env.set]
+
+/--
+`swap` terminates, and the resulting environment contains swapped inputs. This proof is shorter.
+-/
+example : ∃ρ', BigStep (Env.init 0 |>.set "x" 5 |>.set "y" 22) swap ρ' ∧ ρ'.get "x" = 22 ∧ ρ'.get "y" = 5 := by
+  repeat' constructor
+
+/--
+`swap` terminates, and the resulting environment contains swapped inputs. This version works no
+matter what the input values are.
+-/
+example : ∃ρ', BigStep (Env.init 0 |>.set "x" x |>.set "y" y) swap ρ' ∧ ρ'.get "x" = y ∧ ρ'.get "y" = x  := by
+  repeat' constructor
+
+/--
+`min` computes the minimum of its inputs.
+-/
+example : ∃ρ', BigStep (Env.init 0 |>.set "x" x |>.set "y" y) min ρ' ∧ if x < y then ρ'.get "min" = x else ρ'.get "min" = y := by
+  unfold min
+  by_cases h : x < y
+  . apply Exists.intro; constructor
+    . apply BigStep.ifTrue
+      . simp [Expr.eval, Expr.BinOp.apply, Env.get, Env.set, *]; decide
+      . constructor; simp [Expr.eval, Env.get, Env.set]; rfl
+    . simp [Env.get, Env.set]
+      intro; contradiction
+  . apply Exists.intro; constructor
+    . apply BigStep.ifFalse
+      . simp [Expr.eval, Expr.BinOp.apply, Env.get, Env.set, *]
+      . constructor; simp [Expr.eval, Env.get, Env.set]; rfl
+    . simp [Env.get, Env.set]
+      intro; contradiction
+
+
+def loop := imp {while (1) {skip;}}
+
+/--
+`loop` is really an infinite loop - there is no final state that it can result in.
+-/
+theorem infinite_loop : ¬ BigStep ρ loop ρ' := by
+  generalize h' : loop = l
+  intro h
+  induction h with try (simp [loop, *] at *; done)
+  | whileTrue =>
+    simp [*]
+  | whileFalse cFalse =>
+    unfold loop at h'
+    cases h'
+    cases cFalse
+
+def loopOf (s) := imp {while (1) {~s}}
+
+theorem infinite_loopOf : ¬ BigStep ρ (loopOf s) ρ' := by
+  generalize h' : loopOf s = l
+  intro h
+  induction h with try (simp [loopOf, *] at *; done)
+  | whileTrue =>
+    simp [*]
+  | whileFalse cFalse =>
+    unfold loopOf at h'
+    cases h'
+    cases cFalse
+
+
+theorem optimize_ok : BigStep ρ s ρ' → BigStep ρ s.optimize ρ' := by
+  intro h
+  induction h with simp only [optimize]
+  | «skip» => constructor
+  | seq s1 s2 ih1 ih2 =>
+    split
+    next eq2 =>
+      rw [eq2] at ih1
+      cases ih1; apply ih2
+    next eq1 eq2 =>
+      rw [eq1] at ih2
+      cases ih2; apply ih1
+    next =>
+      apply BigStep.seq ih1 ih2
+  | assign m =>
+    constructor
+    rw [← Expr.optimize_ok]
+    assumption
+  | ifTrue isTrue l ih =>
+    split
+    next isFalse =>
+      rw [Expr.optimize_ok] at isTrue
+      rw [isFalse] at isTrue
+      simp [Truthy, Expr.eval] at isTrue
+    next notFalse _isConst =>
+      apply ih
+    next =>
+      split
+      . assumption
+      . apply BigStep.ifTrue
+        . rw [← Expr.optimize_ok]
+          assumption
+        . assumption
+  | ifFalse isFalse l ih =>
+    split
+    next =>
+      apply ih
+    next nonZero isConst =>
+      rw [Expr.optimize_ok, isConst] at isFalse
+      simp at isFalse
+      contradiction
+    next =>
+      split
+      . simp [*]
+      . apply BigStep.ifFalse
+        . rw [← Expr.optimize_ok]
+          assumption
+        . assumption
+  | whileFalse =>
+    split <;> try simp
+    apply BigStep.whileFalse
+    rw [← Expr.optimize_ok]
+    assumption
+  | whileTrue isTrue bodyStep nextStep ih1 ih2 =>
+    split
+    next c isZero =>
+      rw [Expr.optimize_ok, isZero] at isTrue
+      simp at isTrue
+    next c isNotZero =>
+      apply BigStep.whileTrue
+      . rw [← Expr.optimize_ok]
+        assumption
+      . apply ih1
+      . simp [optimize] at ih2
+        assumption
+
+
+inductive BigRes : Nat → Env → Stmt → Type where
+  | done (ρ' : Env) : BigStep ρ s ρ' → BigRes n ρ s
+  | noGas : BigRes n ρ s
+  | crash : ¬(∃ρ', BigStep ρ s ρ') →  BigRes n ρ s
+
+theorem BigStep.no_seq : ¬(∃ ρ', BigStep ρ (imp {~s1 ~s2}) ρ') ↔ ¬(∃ ρ' ρ'', BigStep ρ s1 ρ' ∧ BigStep ρ' s2 ρ'') := by
+  constructor
+  . intro no
+    intro ⟨ρ', ρ'', st1, st2⟩
+    apply no
+    constructor; constructor
+    exact st1
+    exact st2
+  . intro no
+    rintro ⟨ρ', ⟨st1, st2⟩⟩
+    apply no
+    constructor; constructor
+    constructor
+    . assumption
+    . assumption
+
+theorem BigStep.no_assign : ¬(∃ ρ', BigStep ρ (imp {~x := ~e;}) ρ') ↔ e.eval ρ = none := by
+  constructor
+  . intro noSteps
+    cases h : e.eval ρ <;> simp
+    apply noSteps
+    constructor
+    constructor
+    exact h
+  . intro isNone
+    intro h
+    rcases h with ⟨_, ⟨isSome⟩⟩
+    rw [isNone] at *; contradiction
+
+
+def run (ρ : Env) (s : Stmt) : (n : Nat) → BigRes n ρ s
+  | 0 => .noGas
+  | n + 1 =>
+    match s with
+    | imp {skip;} =>
+      .done ρ .skip
+    | imp {~s1 ~s2} =>
+      match run ρ s1 n with
+      | .done ρ' st1 =>
+        match run ρ' s2 n with
+        | .done ρ'' st2 => .done ρ'' (.seq st1 st2)
+        | .noGas => .noGas
+        | .crash no => .crash <| by
+          rw [BigStep.no_seq]
+          rintro ⟨ρ', ρ'', st1', st2'⟩
+          apply no
+          have := BigStep.unique st1 st1'
+          subst this
+          constructor; assumption
+      | .noGas => .noGas
+      | .crash no => .crash <| by
+        rw [BigStep.no_seq]
+        intro h
+        simp at h
+        apply no
+        rcases h with ⟨_, _, ⟨_, _⟩⟩
+        constructor; assumption
+    | imp {~x := ~e;} =>
+      match h : e.eval ρ with
+      | none => .crash <| by
+        rw [BigStep.no_assign]
+        simp [*]
+      | some v => .done _ (.assign h)
+    | imp {if (~c) {~s1} else {~s2}} =>
+      match h : c.eval ρ with
+      | none => .crash <| by
+        intro ⟨ρ', st⟩
+        cases st with
+        | ifTrue =>
+          simp [*] at *
+        | ifFalse =>
+          simp [*] at *
+      | some v =>
+        if h' : v = 0 then
+          match run ρ s2 n with
+          | .done ρ' step => .done ρ' (.ifFalse (by simp [h, h']) step)
+          | .noGas => .noGas
+          | .crash no => .crash <| by
+            intro ⟨ρ', st⟩
+            apply no
+            cases st with
+            | ifTrue isTrue step1 =>
+              have := isTrue.not_falsy
+              simp [*] at *
+            | ifFalse isFalse step2 =>
+              constructor; assumption
+        else
+          match run ρ s1 n with
+          | .done ρ' step => .done ρ' (.ifTrue (by simp [h, h']; assumption) step)
+          | .noGas => .noGas
+          | .crash no => .crash <| by
+            intro ⟨ρ', st⟩
+            apply no
+            cases st with
+            | ifTrue isTrue step1 =>
+              constructor; assumption
+            | ifFalse isFalse step2 =>
+              simp [Falsy, h, h'] at isFalse
+              contradiction
+    | imp {while (~c) {~s1}} =>
+      match h : c.eval ρ with
+      | none => .crash <| by
+        intro ⟨ρ', st⟩
+        cases st <;> simp [*] at *
+      | some v =>
+        if h' : v = 0 then
+          .done _ <| .whileFalse (by simp [*])
+        else
+          have truthy : Truthy (c.eval ρ) := by simp [*]; assumption
+          match run ρ s1 n with
+          | .done ρ' step =>
+            match run ρ' (imp {while (~c) {~s1}}) n with
+            | .done ρ'' step' =>
+              .done ρ'' (.whileTrue truthy step step')
+            | .noGas => .noGas
+            | .crash no =>
+              .crash <| by
+                intro ⟨ρ'', st⟩
+                cases st
+                . have := BigStep.unique step (by assumption)
+                  subst this
+                  apply no
+                  constructor; assumption
+                . simp [*] at *; contradiction
+          | .noGas => .noGas
+          | .crash no => .crash <| by
+            intro ⟨ρ', st⟩
+            cases st with
+            | whileFalse =>
+              simp [*] at *; contradiction
+            | whileTrue =>
+              apply no
+              constructor; assumption
+
+def run' (ρ : Env) (s : Stmt) : (n : Nat) → Option Env
+  | 0 => none
+  | n + 1 =>
+    match s with
+    | imp {skip;} =>
+      some ρ
+    | imp {~s1 ~s2} => do
+      let ρ' ← run' ρ s1 n
+      run' ρ' s2 n
+    | imp {~x := ~e;} => do
+      let v ← e.eval ρ
+      pure (ρ.set x v)
+    | imp {if (~c) {~s1} else {~s2}} => do
+      let v ← c.eval ρ
+      if v = 0 then
+        run' ρ s2 n
+      else
+        run' ρ s1 n
+    | imp {while (~c) {~s1}} => do
+      let v ← c.eval ρ
+      if v = 0 then
+        pure ρ
+      else
+        let ρ' ← run' ρ s1 n
+        run' ρ' (imp {while (~c) {~s1}}) n
+
+
+def terminatesWith (n : Nat) (ρ : Env) (s : Stmt) : Option Env :=
+  match run ρ s n with
+  | .done ρ' _ => some ρ'
+  | _ => none
